dist/Klas_Arange.h
@@ -1,0 +1,10 @@
+
+#ifndef Klas_Arange_H
+#define Klas_Arange_H
+
+#include <kuiper.h>
+
+uint64_t *Klas_Arange_arange_i64(uint32_t n, uint64_t start, uint64_t step);
+
+#define Klas_Arange_H_DEFINED
+#endif                          /* Klas_Arange_H */
