dist/Klas_CatCast.h
@@ -4,8 +4,9 @@
 
 #include <kuiper.h>
 
-__nv_bfloat16 *Klas_CatCast_cat2_bf16(uint32_t len, __nv_bfloat16 * a,
-                                      __nv_bfloat16 * b);
+__nv_bfloat16
+    * Klas_CatCast_cat2_bf16(uint32_t lena, uint32_t lenb, __nv_bfloat16 * a,
+                             __nv_bfloat16 * b);
 
 float *Klas_CatCast_cast_bf16_to_f32(uint32_t len, __nv_bfloat16 * a);
 
