dist/Klas_Misc.h
@@ -1,8 +1,0 @@
-
-#ifndef Klas_Misc_H
-#define Klas_Misc_H
-
-#include <kuiper.h>
-
-#define Klas_Misc_H_DEFINED
-#endif                          /* Klas_Misc_H */
