dist/Klas_Reduce.cu
@@ -1,61 +1,43 @@
 
 #include "Klas_Reduce.h"
 
-typedef struct __uint32_t__uint32_t_______s {
-    uint32_t fst;
-    uint32_t snd;
-} __uint32_t__uint32_t______;
-
 __global__
 /**
-  hoisted when extracting mean_fw_f32_row
+  hoisted when extracting mean
 */
-static void __hoisted_mean_fw_f32_row_0(uint32_t cols, float *x, float *y)
+static void __hoisted_mean_0(uint32_t n, float *a, float *out)
 {
-    float *sa = (float *)KPR_SHMEM_AT(0U);
+    float *sa1 = (float *)KPR_SHMEM_AT(0U);
     float acc = 0.0f;
     uint32_t idx = threadIdx.x;
-    for (; idx < cols; idx += 1024U) {
-        __uint32_t__uint32_t______ scrut = {.fst = blockIdx.x,.snd = idx };
-        acc += x[scrut.fst * cols + scrut.snd];
-    }
-    sa[threadIdx.x] = acc;
-    uint32_t n = 0U;
-    for (; 1U << (uint32_t) n < 1024U; n++) {
-        uint32_t __anf01 = n;
+    for (; idx < n; idx += 1024U)
+        acc += a[idx];
+    sa1[threadIdx.x] = acc;
+    uint32_t n1 = 0U;
+    for (; 1U << (uint32_t) n1 < 1024U; n1++) {
+        uint32_t __anf01 = n1;
         __syncthreads();
         uint32_t nextid = threadIdx.x + (uint32_t) (1U << (uint32_t) __anf01);
         if (nextid < 1024U)
             if ((threadIdx.x & (uint32_t) (1U << (uint32_t) (__anf01 + 1U)) -
                  1U) == 0U)
-                sa[threadIdx.x] += sa[nextid];
+                sa1[threadIdx.x] += sa1[nextid];
     }
     if (threadIdx.x == 0U)
-        y[blockIdx.x] = *sa;
+        *out = *sa1;
 }
 
-__global__
-/**
-  hoisted when extracting mean_fw_f32_row
-*/
-static void __hoisted_mean_fw_f32_row_1(uint32_t rows, float inv_cols, float *y)
+float Klas_Reduce_mean(uint32_t n, float *a)
 {
-    if (1024U * blockIdx.x + threadIdx.x < rows)
-        y[1024U * blockIdx.x + threadIdx.x] *= inv_cols;
-}
-
-void
-Klas_Reduce_mean_fw_f32_row(uint32_t rows, uint32_t cols, float inv_cols,
-                            float *x, float *y)
-{
+    float *out = (float *)KPR_GPU_ALLOC(sizeof(float), 1U);
     KPR_SHMEM_FITS(4096U);
-    MUST(cudaFuncSetAttribute(__hoisted_mean_fw_f32_row_0,
-                              cudaFuncAttributeMaxDynamicSharedMemorySize,
-                              4096U));
-    KPR_KCALL(__hoisted_mean_fw_f32_row_0, rows, 1024U, 4096U, cols, x, y);
+    MUST(cudaFuncSetAttribute
+         (__hoisted_mean_0, cudaFuncAttributeMaxDynamicSharedMemorySize,
+          4096U));
+    KPR_KCALL(__hoisted_mean_0, 1U, 1024U, 4096U, n, a, out);
     MUST(cudaDeviceSynchronize());
-    KPR_KCALL(__hoisted_mean_fw_f32_row_1,
-              rows / 1024U + (uint32_t) (rows % 1024U != 0U),
-              1024U, 0U, rows, inv_cols, y);
-    MUST(cudaDeviceSynchronize());
+    float hout = 0.0f;
+    MUST(cudaMemcpy(&hout, out, sizeof(float), cudaMemcpyDeviceToHost));
+    MUST(cudaFree(out));
+    return hout / (float)(int64_t) (uint32_t) n;
 }
