src/klas/Klas.Reduce.fst
@@ -3,66 +3,29 @@ module Klas.Reduce
 #lang-pulse
 
 open Kuiper
-open Kuiper.Tensor { ctlayout }
 open Kuiper.Tensor.Layout.Alg
 open Kuiper.Seq.Common
 module Array1 = Kuiper.Array1
-module Array2 = Kuiper.Array2
-module EM = Kuiper.EMatrix
 module SZ = Kuiper.SizeT
-module HRedB = Kuiper.Kernel.HReduce.Block
-module Map = Kuiper.Kernel.Map
+module HReduce = Kuiper.Kernel.HReduce
 
-let mean_row_aux
-  (#rows #cols : nat)
-  (inv_cols : f32)
-  (sx : EM.ematrix f32 rows cols)
-  (s_sum : lseq f32 rows)
-  (r : nat { r < rows })
-  : Lemma
-      (requires (s_sum @! r) %~ rsum (lseq_map id (EM.ematrix_row (EM.to_real_matrix sx) r)))
-      (ensures
-        (exists (sumr : f32).
-          sumr %~ rsum (lseq_map id (EM.ematrix_row (EM.to_real_matrix sx) r)) /\
-          (lseq_map (mean_scale inv_cols) s_sum) @! r == mean_scale inv_cols sumr))
-  = assert ((lseq_map (mean_scale inv_cols) s_sum) @! r == mean_scale inv_cols (s_sum @! r))
-
-#push-options "--z3rlimit 80"
-inline_for_extraction noextract
-fn mean_fw_f32_row_impl
-  (rows : szp { rows <= max_blocks })
-  (cols : szp { SZ.fits (cols + max_threads) })
-  (inv_cols : f32)
-  (x : Array2.t f32 (l2_row_major rows cols) { Array2.is_global x })
-  (y : Array1.t f32 (l1_forward rows) { Array1.is_global y })
-  (#sx : erased (EM.ematrix f32 rows cols))
-  (#sy : erased (lseq f32 rows))
+fn mean
+  (n : szp { SZ.fits (n + max_threads) })
+  (a : Array1.t f32 (l1_forward n) { Array1.is_global a })
+  (#sa : erased (lseq f32 n))
   preserves cpu
-  requires
-    on gpu_loc (x |-> sx) **
-    on gpu_loc (y |-> sy)
-  ensures
-    on gpu_loc (x |-> sx) **
-    (exists* (sy' : lseq f32 rows).
-       on gpu_loc (y |-> sy') **
-       pure (mean_fw_f32_row_post rows cols inv_cols (reveal sx) sy'))
+  preserves on gpu_loc (a |-> sa)
+  returns res : f32
+  ensures pure (res %~ (rsum (to_real_seq (reveal sa)) /. Real.of_int n))
 {
-  let vr : erased (EM.ematrix real rows cols) = hide (EM.to_real_matrix (reveal sx));
-  EM.lemma_to_real_matrix_approximates (reveal sx);
-  HRedB.reduce_batched_block #f32 id id rows cols 1024sz
-    #_ #(c_l2_row_major _ _)
-    #_ #(c_l1_forward _)
-    x y (reveal vr);
-  with sy1. assert (on gpu_loc (y |-> sy1));
-
-  assert pure (rows <= max_blocks * max_threads);
-  Map.map_gpu (mean_scale inv_cols) rows #_ #(c_l1_forward _) y;
-
-  Classical.forall_intro
-    (Classical.move_requires
-       (mean_row_aux inv_cols (reveal sx) (reveal sy1)));
-  ()
+  let vr : erased (lseq real n) = hide (to_real_seq (reveal sa));
+  to_real_seq_is_approx (reveal sa);
+  let sum : f32 =
+    HReduce.reduce #f32 id id 1024sz n #(l1_forward n) #(c_l1_forward _) a vr;
+  assert pure (Seq.equal (seq_map id (reveal vr)) (reveal vr));
+  let n_u32 : FStar.UInt32.t = SZ.sizet_to_u32 n;
+  let n_i64 : FStar.Int64.t = FStar.Int.Cast.uint32_to_int64 n_u32;
+  let nf : f32 = of_int #f32 n_i64;
+  of_int_approx #f32 n_i64;
+  div sum nf
 }
-#pop-options
-
-let mean_fw_f32_row : mean_fw_f32_row_ty = mean_fw_f32_row_impl
