src/klas/Klas.CatCast.fst
@@ -5,33 +5,28 @@ open Kuiper
 
 module Array1 = Kuiper.Array1
 module Map = Kuiper.Kernel.Map
+module Cat = Kuiper.Kernel.Cat
 module Casts = Kuiper.Float.Casts.Base
 module SZ = Kuiper.SizeT
 open Kuiper.Tensor.Layout.Alg
 
-let cat2_seq
-  #et
-  #len
-  (sa : lseq et len)
-  (sb : lseq et len)
-  : GTot (lseq et (len + len))
-  = Seq.init_ghost (len + len) (fun i -> if i < len then sa @! i else sb @! (i - len))
-
 fn cat2_bf16
-  (len : szp { SZ.fits (len + len) /\ len + len <= max_blocks * max_threads })
-  (a : Array1.t bf16 (l1_forward len) { Array1.is_global a })
-  (b : Array1.t bf16 (l1_forward len) { Array1.is_global b })
-  (#sa #sb : erased (lseq bf16 len))
+  (lena : szp)
+  (lenb : szp { SZ.fits (lena + lenb) /\ lena + lenb <= max_blocks * max_threads })
+  (a : Array1.t bf16 (l1_forward lena) { Array1.is_global a })
+  (b : Array1.t bf16 (l1_forward lenb) { Array1.is_global b })
+  (#sa : erased (lseq bf16 lena))
+  (#sb : erased (lseq bf16 lenb))
   (#fa #fb : perm)
   norewrite
-  preserves
-    cpu **
-    on gpu_loc (a |-> Frac fa sa) **
-    on gpu_loc (b |-> Frac fb sb)
-  returns c : Array1.t bf16 (l1_forward (len + len))
-  ensures exists* sc. on gpu_loc (c |-> sc) ** pure (Array1.is_global c)
+  preserves cpu
+  preserves on gpu_loc (a |-> Frac fa sa) ** on gpu_loc (b |-> Frac fb sb)
+  returns c : Array1.t bf16 (l1_forward (lena + lenb))
+  ensures
+    on gpu_loc (c |-> (Cat.cat2_seq sa sb <: lseq bf16 (lena + lenb))) **
+    pure (Array1.is_global c)
 {
-  Array1.alloc0 #bf16 (len +^ len) (l1_forward (len +^ len))
+  Cat.cat2_gpu lena lenb a b
 }
 
 inline_for_extraction noextract
@@ -45,11 +40,12 @@ fn cast
   norewrite
   preserves cpu ** on gpu_loc (a |-> Frac fa sa)
   returns c : Array1.t ot (l1_forward len)
-  ensures exists* sc. on gpu_loc (c |-> sc) ** pure (Array1.is_global c)
+  ensures
+    on gpu_loc (c |-> (Kuiper.Seq.Common.lseq_map f sa <: lseq ot len)) **
+    pure (Array1.is_global c)
 {
   let c = Array1.alloc0 #ot len (l1_forward len);
-  with sc. assert on gpu_loc (c |-> sc);
-  Map.map_gpu_cast f len a c #_ #_ #sa #sc #fa;
+  Map.map_gpu_notinplace f len a c;
   c
 }
 
@@ -61,9 +57,11 @@ fn cast_bf16_to_f32
   norewrite
   preserves cpu ** on gpu_loc (a |-> Frac fa sa)
   returns c : Array1.t f32 (l1_forward len)
-  ensures exists* sc. on gpu_loc (c |-> sc) ** pure (Array1.is_global c)
+  ensures
+    on gpu_loc (c |-> (Kuiper.Seq.Common.lseq_map Casts.cast_bf16_to_f32 sa <: lseq f32 len)) **
+    pure (Array1.is_global c)
 {
-  cast #bf16 #f32 Casts.cast_bf16_to_f32 len a #sa #fa
+  cast #bf16 #f32 Casts.cast_bf16_to_f32 len a
 }
 
 fn cast_f32_to_bf16
@@ -74,9 +72,11 @@ fn cast_f32_to_bf16
   norewrite
   preserves cpu ** on gpu_loc (a |-> Frac fa sa)
   returns c : Array1.t bf16 (l1_forward len)
-  ensures exists* sc. on gpu_loc (c |-> sc) ** pure (Array1.is_global c)
+  ensures
+    on gpu_loc (c |-> (Kuiper.Seq.Common.lseq_map Casts.cast_f32_to_bf16 sa <: lseq bf16 len)) **
+    pure (Array1.is_global c)
 {
-  cast #f32 #bf16 Casts.cast_f32_to_bf16 len a #sa #fa
+  cast #f32 #bf16 Casts.cast_f32_to_bf16 len a
 }
 
 fn cast_bf16_to_bf16
@@ -87,7 +87,9 @@ fn cast_bf16_to_bf16
   norewrite
   preserves cpu ** on gpu_loc (a |-> Frac fa sa)
   returns c : Array1.t bf16 (l1_forward len)
-  ensures exists* sc. on gpu_loc (c |-> sc) ** pure (Array1.is_global c)
+  ensures
+    on gpu_loc (c |-> (Kuiper.Seq.Common.lseq_map id sa <: lseq bf16 len)) **
+    pure (Array1.is_global c)
 {
-  cast #bf16 #bf16 id len a #sa #fa
+  cast #bf16 #bf16 id len a
 }
